examples/ProcThreeStDec.v
@@ -3,12 +3,14 @@ Require Import Lib.CommonTactics Lib.ilist Lib.Word.
 Require Import Lib.Struct Lib.StructNotation Lib.StringBound Lib.FMap Lib.StringEq Lib.Indexer.
 Require Import Kami.Syntax Kami.Semantics Kami.RefinementFacts Kami.Renaming Kami.Wf.
 Require Import Kami.Renaming Kami.Inline Kami.InlineFacts.
-Require Import Kami.Decomposition Kami.Notations Kami.Tactics Kami.ModuleBoundEx.
+Require Import Kami.Decomposition Kami.Notations Kami.Tactics.
 Require Import Ex.MemTypes Ex.NativeFifo Ex.MemAtomic.
-Require Import Ex.SC Ex.ProcDec Ex.ProcTwoStage Ex.ProcTwoStDec Ex.ProcFDCorrect.
+Require Import Ex.SC Ex.ProcDec Ex.ProcThreeStage Ex.ProcThreeStInl Ex.ProcThreeStInv.
 Require Import Eqdep.
 
-Section ProcFDE.
+Set Implicit Arguments.
+
+Section ProcThreeStDec.
   Variables addrSize lgDataBytes rfIdx: nat.
 
   (* External abstract ISA: decoding and execution *)
@@ -29,7 +31,6 @@ Section ProcFDE.
             (predictNextPc: forall ty, fullType ty (SyntaxKind (Bit addrSize)) -> (* pc *)
                                        Expr ty (SyntaxKind (Bit addrSize))).
 
-  (* Abstract d2eElt *)
   Variable (d2eElt: Kind).
   Variable (d2ePack:
               forall ty,
@@ -61,26 +62,26 @@ Section ProcFDE.
     (d2eEpoch: forall ty, fullType ty (SyntaxKind d2eElt) ->
                           Expr ty (SyntaxKind Bool)).
 
-  (* Abstract f2dElt *)  
-  Variable (f2dElt: Kind).
-  Variable (f2dPack:
-              forall ty,
-                Expr ty (SyntaxKind (Data lgDataBytes)) -> (* rawInst *)
-                Expr ty (SyntaxKind (Bit addrSize)) -> (* curPc *)
-                Expr ty (SyntaxKind (Bit addrSize)) -> (* nextPc *)
-                Expr ty (SyntaxKind Bool) -> (* epoch *)
-                Expr ty (SyntaxKind f2dElt)).
-  Variables
-    (f2dRawInst: forall ty, fullType ty (SyntaxKind f2dElt) ->
-                            Expr ty (SyntaxKind (Data lgDataBytes)))
-    (f2dCurPc: forall ty, fullType ty (SyntaxKind f2dElt) ->
-                          Expr ty (SyntaxKind (Bit addrSize)))
-    (f2dNextPc: forall ty, fullType ty (SyntaxKind f2dElt) ->
-                           Expr ty (SyntaxKind (Bit addrSize)))
-    (f2dEpoch: forall ty, fullType ty (SyntaxKind f2dElt) ->
-                          Expr ty (SyntaxKind Bool)).
+  Hypotheses
+    (Hd2eOpType: forall opType dst addr val1 val2 rawInst curPc nextPc epoch,
+        evalExpr (d2eOpType _ (evalExpr (d2ePack opType dst addr val1 val2 rawInst curPc nextPc epoch))) = evalExpr opType)
+    (Hd2eDst: forall opType dst addr val1 val2 rawInst curPc nextPc epoch,
+        evalExpr (d2eDst _ (evalExpr (d2ePack opType dst addr val1 val2 rawInst curPc nextPc epoch))) = evalExpr dst)
+    (Hd2eAddr: forall opType dst addr val1 val2 rawInst curPc nextPc epoch,
+        evalExpr (d2eAddr _ (evalExpr (d2ePack opType dst addr val1 val2 rawInst curPc nextPc epoch))) = evalExpr addr)
+    (Hd2eVal1: forall opType dst addr val1 val2 rawInst curPc nextPc epoch,
+        evalExpr (d2eVal1 _ (evalExpr (d2ePack opType dst addr val1 val2 rawInst curPc nextPc epoch))) = evalExpr val1)
+    (Hd2eVal2: forall opType dst addr val1 val2 rawInst curPc nextPc epoch,
+        evalExpr (d2eVal2 _ (evalExpr (d2ePack opType dst addr val1 val2 rawInst curPc nextPc epoch))) = evalExpr val2)
+    (Hd2eRawInst: forall opType dst addr val1 val2 rawInst curPc nextPc epoch,
+        evalExpr (d2eRawInst _ (evalExpr (d2ePack opType dst addr val1 val2 rawInst curPc nextPc epoch))) = evalExpr rawInst)
+    (Hd2eCurPc: forall opType dst addr val1 val2 rawInst curPc nextPc epoch,
+        evalExpr (d2eCurPc _ (evalExpr (d2ePack opType dst addr val1 val2 rawInst curPc nextPc epoch))) = evalExpr curPc)
+    (Hd2eNextPc: forall opType dst addr val1 val2 rawInst curPc nextPc epoch,
+        evalExpr (d2eNextPc _ (evalExpr (d2ePack opType dst addr val1 val2 rawInst curPc nextPc epoch))) = evalExpr nextPc)
+    (Hd2eEpoch: forall opType dst addr val1 val2 rawInst curPc nextPc epoch,
+        evalExpr (d2eEpoch _ (evalExpr (d2ePack opType dst addr val1 val2 rawInst curPc nextPc epoch))) = evalExpr epoch).
 
-  (* Abstract e2wElt *)  
   Variable (e2wElt: Kind).
   Variable (e2wPack:
               forall ty,
@@ -93,41 +94,217 @@ Section ProcFDE.
     (e2wVal: forall ty, fullType ty (SyntaxKind e2wElt) ->
                         Expr ty (SyntaxKind (Data lgDataBytes))).
 
-  Definition fetchDecode := ProcFetchDecode.fetchDecode
-                              getOptype getLdDst getLdAddr getLdSrc calcLdAddr
-                              getStAddr getStSrc calcStAddr getStVSrc
-                              getSrc1 getSrc2 getDst predictNextPc d2ePack
-                              f2dPack f2dRawInst f2dCurPc f2dNextPc f2dEpoch.
+  Hypotheses
+    (He2wDecInst: forall decInst val,
+        evalExpr (e2wDecInst _ (evalExpr (e2wPack decInst val))) = evalExpr decInst)
+    (He2wVal: forall decInst val,
+        evalExpr (e2wVal _ (evalExpr (e2wPack decInst val))) = evalExpr val).
 
-  Definition p3st := (fetchDecode
-                        ++ regFile lgDataBytes rfIdx
-                        ++ scoreBoard rfIdx
-                        ++ oneEltFifo d2eFifoName d2eElt
-                        ++ oneEltFifoEx1 e2dFifoName (Bit addrSize)
-                        ++ (executer rfIdx exec d2eOpType d2eVal1 d2eVal2
-                                     d2eRawInst d2eCurPc e2wPack)
-                        ++ epoch
-                        ++ oneEltFifo e2wFifoName e2wElt
-                        ++ (wb "rqFromProc"%string "rsToProc"%string
-                               getNextPc d2eOpType d2eDst d2eAddr d2eVal1 d2eRawInst
-                               d2eCurPc d2eNextPc d2eEpoch e2wDecInst e2wVal))%kami.
+  Definition p3st := ProcThreeStage.p3st
+                       getOptype getLdDst getLdAddr getLdSrc calcLdAddr
+                       getStAddr getStSrc calcStAddr getStVSrc
+                       getSrc1 getSrc2 getDst exec getNextPc predictNextPc
+                       d2ePack d2eOpType d2eDst d2eAddr d2eVal1 d2eVal2
+                       d2eRawInst d2eCurPc d2eNextPc d2eEpoch
+                       e2wPack e2wDecInst e2wVal.
+  Definition pdec := ProcDec.pdec
+                       getOptype getLdDst getLdAddr getLdSrc calcLdAddr
+                       getStAddr getStSrc calcStAddr getStVSrc
+                       getSrc1 getSrc2 getDst exec getNextPc.
+  
+  Hint Unfold p3st: ModuleDefs. (* for kinline_compute *)
+  Hint Extern 1 (ModEquiv type typeUT p3st) => unfold p3st. (* for kequiv *)
+  Hint Extern 1 (ModEquiv type typeUT pdec) => unfold pdec. (* for kequiv *)
 
-  Definition p2st := ProcTwoStage.p2st getOptype getLdDst getLdAddr getLdSrc calcLdAddr
-                                       getStAddr getStSrc calcStAddr getStVSrc
-                                       getSrc1 getSrc2 getDst exec getNextPc predictNextPc
-                                       d2ePack d2eOpType d2eDst d2eAddr d2eVal1 d2eVal2
-                                       d2eRawInst d2eCurPc d2eNextPc d2eEpoch
-                                       e2wPack e2wDecInst e2wVal.
+  Definition p3st_pdec_ruleMap (o: RegsT): string -> option string :=
+    "reqLd" |-> "reqLd";
+      "reqLdZ" |-> "reqLdZ";
+      "reqSt" |-> "reqSt";
+      "repLd" |-> "repLd";
+      "repSt" |-> "repSt";
+      "execToHost" |-> "execToHost";
+      "wbNm" |-> "execNm"; ||.
+  Hint Unfold p3st_pdec_ruleMap: MethDefs.
 
-  Lemma p3st_refines_p2st: p3st <<== p2st.
+  Definition p3st_pdec_regMap (r: RegsT): RegsT :=
+    (mlet pcv : (Bit addrSize) <- r |> "pc";
+       mlet pgmv : (Vector (Data lgDataBytes) addrSize) <- r |> "pgm";
+       mlet rfv : (Vector (Data lgDataBytes) rfIdx) <- r |> "rf";
+       mlet d2eeltv : d2eElt <- r |> "d2e"--"elt";
+       mlet d2efv : Bool <- r |> "d2e"--"full";
+       mlet e2weltv : e2wElt <- r |> "e2w"--"elt";
+       mlet e2wfv : Bool <- r |> "e2w"--"full";
+       mlet w2deltv : Bit addrSize <- r |> "w2d"--"elt";
+       mlet w2dfv : Bool <- r |> "w2d"--"full";
+       mlet eev : Bool <- r |> "eEpoch";
+       mlet stallv : Bool <- r |> "stall";
+       mlet stalledv : d2eElt <- r |> "stalled";
+
+       (["stall" <- existT _ _ stallv]
+        +["pgm" <- existT _ _ pgmv]
+        +["rf" <- existT _ _ rfv]
+        +["pc" <- existT _ (SyntaxKind (Bit addrSize))
+               (if w2dfv then w2deltv
+                else if stallv then evalExpr (d2eCurPc _ stalledv)
+                     else if e2wfv then
+                            (if eqb eev (evalExpr (d2eEpoch _ (evalExpr (e2wDecInst _ e2weltv))))
+                             then evalExpr (d2eCurPc _ (evalExpr (e2wDecInst _ e2weltv)))
+                             else
+                               (if d2efv then
+                                 (if eqb eev (evalExpr (d2eEpoch _ d2eeltv))
+                                  then evalExpr (d2eCurPc _ d2eeltv)
+                                  else pcv)
+                                else pcv))
+                          else if d2efv then
+                                 (if eqb eev (evalExpr (d2eEpoch _ d2eeltv))
+                                  then evalExpr (d2eCurPc _ d2eeltv)
+                                  else pcv)
+                               else pcv)])%fmap)%mapping.
+  Hint Unfold p3st_pdec_regMap: MapDefs.
+
+  Ltac is_not_ife t :=
+    match t with
+    | context [if _ then _ else _] => fail 1
+    | _ => idtac
+    end.
+  
+  Ltac dest_if :=
+    match goal with
+    | [ |- context[if ?x then _ else _] ] =>
+      let c := fresh "c" in is_not_ife x; remember x as c; destruct c
+    | [H: context[if ?x then _ else _] |- _] =>
+      let c := fresh "c" in is_not_ife x; remember x as c; destruct c
+    end.
+
+  Ltac d2e_abs_tac :=
+    try rewrite Hd2eOpType in *;
+    try rewrite Hd2eDst in *;
+    try rewrite Hd2eAddr in *;
+    try rewrite Hd2eVal1 in *;
+    try rewrite Hd2eVal2 in *;
+    try rewrite Hd2eRawInst in *;
+    try rewrite Hd2eCurPc in *;
+    try rewrite Hd2eNextPc in *;
+    try rewrite Hd2eEpoch in *;
+    try rewrite He2wDecInst in *;
+    try rewrite He2wVal in *.
+
+  Ltac kinv_bool :=
+    repeat
+      (try match goal with
+           | [H: ?t = true |- _] => rewrite H in *
+           | [H: ?t = false |- _] => rewrite H in *
+           | [H: true = ?t |- _] => rewrite <-H in *
+           | [H: false = ?t |- _] => rewrite <-H in *
+           end; dest_if; kinv_simpl; intuition idtac).
+
+  Ltac p3st_inv_tac :=
+    repeat match goal with
+           | [H: context[p3st_epochs_inv] |- _] => destruct H
+           | [H: context[p3st_pc_inv] |- _] => destruct H
+           | [H: context[p3st_decode_inv] |- _] => destruct H
+           | [H: context[p3st_stalled_inv] |- _] => destruct H
+           | [H: context[p3st_raw_inv] |- _] => destruct H
+           | [H: context[p3st_scoreboard_waw_inv] |- _] => destruct H
+           | [H: context[p3st_exec_inv] |- _] => destruct H
+           end;
+    kinv_red.
+
+  Definition p3stInl := ProcThreeStInl.p3stInl getOptype getLdDst getLdAddr getLdSrc calcLdAddr
+                                               getStAddr getStSrc calcStAddr getStVSrc
+                                               getSrc1 getSrc2 getDst exec getNextPc predictNextPc
+                                               d2ePack d2eOpType d2eDst d2eAddr d2eVal1 d2eVal2
+                                               d2eRawInst d2eCurPc d2eNextPc d2eEpoch
+                                               e2wPack e2wDecInst e2wVal.
+
+  Theorem p3st_refines_pdec:
+    p3st <<== pdec.
   Proof. (* SKIP_PROOF_ON
-    kmodular.
-    - kdisj_edms_cms_ex O.
-    - kdisj_ecms_dms_ex O.
-    - apply fetchDecode_refines_fetchNDecode.
-    - krefl.
+    (* instead of: kinline_left im. *)
+    ketrans; [exact (projT2 p3stInl)|].
+    kdecompose_nodefs p3st_pdec_regMap p3st_pdec_ruleMap.
+
+    kinv_add p3st_inv_ok.
+    kinv_add_end.
+
+    kinvert.
+    - kinv_action_dest;
+        kinv_custom p3st_inv_tac;
+        kinv_regmap_red;
+        kinv_constr; kinv_eq; d2e_abs_tac; kinv_finish_with kinv_bool.
+    - kinv_action_dest;
+        kinv_custom p3st_inv_tac;
+        kinv_regmap_red;
+        kinv_constr; kinv_eq; d2e_abs_tac; kinv_finish_with kinv_bool.
+    - kinv_action_dest;
+        kinv_custom p3st_inv_tac;
+        kinv_regmap_red;
+        kinv_constr; kinv_eq; d2e_abs_tac; kinv_finish_with kinv_bool.
+    - kinv_action_dest;
+        kinv_custom p3st_inv_tac;
+        kinv_regmap_red;
+        kinv_constr; kinv_eq; d2e_abs_tac; kinv_finish_with kinv_bool.
+    - kinv_action_dest;
+        kinv_custom p3st_inv_tac;
+        kinv_regmap_red;
+        kinv_constr; kinv_eq; d2e_abs_tac; kinv_finish_with kinv_bool.
+    - kinv_action_dest;
+        kinv_custom p3st_inv_tac;
+        kinv_regmap_red;
+        kinv_constr; kinv_eq; d2e_abs_tac; kinv_finish_with kinv_bool.
+    - kinv_action_dest;
+        kinv_custom p3st_inv_tac;
+        kinv_regmap_red;
+        kinv_constr; kinv_eq; d2e_abs_tac; kinv_finish_with kinv_bool.
+    - kinv_action_dest;
+        kinv_custom p3st_inv_tac;
+        kinv_regmap_red;
+        kinv_constr; kinv_eq; d2e_abs_tac; kinv_finish_with kinv_bool.
+    - kinv_action_dest;
+        kinv_custom p3st_inv_tac;
+        kinv_regmap_red;
+        kinv_constr;
+        try (kinv_eq; d2e_abs_tac; kinv_finish_with kinv_bool; fail).
+      Opaque evalExpr.
+      kinv_eq; d2e_abs_tac; kinv_finish_with kinv_bool.
+      Transparent evalExpr.
+    - kinv_action_dest;
+        kinv_custom p3st_inv_tac;
+        kinv_regmap_red;
+        kinv_constr;
+        kinv_eq; d2e_abs_tac; kinv_finish_with kinv_bool.
+    - kinv_action_dest;
+        kinv_custom p3st_inv_tac;
+        kinv_regmap_red;
+        kinv_constr;
+        try (kinv_eq; d2e_abs_tac; kinv_finish_with kinv_bool; fail).
+      Opaque evalExpr.
+      kinv_eq; d2e_abs_tac; kinv_finish_with kinv_bool.
+      Transparent evalExpr.
+    - kinv_action_dest;
+        kinv_custom p3st_inv_tac;
+        kinv_regmap_red;
+        kinv_constr;
+        kinv_eq; d2e_abs_tac; kinv_finish_with kinv_bool.
+    - kinv_action_dest;
+        kinv_custom p3st_inv_tac;
+        kinv_regmap_red;
+        kinv_constr;
+        kinv_eq; d2e_abs_tac; kinv_finish_with kinv_bool.
+    - kinv_action_dest;
+        kinv_custom p3st_inv_tac;
+        kinv_regmap_red;
+        kinv_constr;
+        kinv_eq; d2e_abs_tac; kinv_finish_with kinv_bool.
+    - kinv_action_dest;
+        kinv_custom p3st_inv_tac;
+        kinv_regmap_red;
+        kinv_constr;
+        kinv_eq; d2e_abs_tac; kinv_finish_with kinv_bool.
+
       END_SKIP_PROOF_ON *) admit.
+
   Qed.
 
-End ProcFDE.
+End ProcThreeStDec.
 
