extraction/Extraction.v
@@ -16,8 +16,8 @@ Unset Extraction AutoInline.
 Require Import Kami.Syntax Kami.ParametricSyntax Kami.Duplicate
         Kami.Notations Kami.Synthesize Ex.Isa.
 
-(** p2st + memAtomic test *)
-Require Import Ex.ProcTwoStage Ex.ProcTwoStDec Ex.MemAtomic.
+(** p4st + memAtomic test *)
+Require Import Ex.ProcFetchDecode Ex.ProcThreeStage Ex.ProcFourStDec Ex.MemAtomic.
 
 (* AddrSize = IdxBits + TagBits + LgNumDatas *)
 Definition idxBits := 2.
@@ -31,19 +31,23 @@ Definition idK := Bit 1.
 Definition predictNextPc ty (ppc: fullType ty (SyntaxKind (Bit rv32iAddrSize))) :=
   (#ppc + $1)%kami_expr.
 
-Definition p2st := p2st rv32iGetOptype
+Definition p4st := p4st rv32iGetOptype
                         rv32iGetLdDst rv32iGetLdAddr rv32iGetLdSrc rv32iCalcLdAddr
                         rv32iGetStAddr rv32iGetStSrc rv32iCalcStAddr rv32iGetStVSrc
                         rv32iGetSrc1 rv32iGetSrc2 rv32iGetDst rv32iExec rv32iNextPc
                         predictNextPc (@d2ePackI _ _ _)
-                        (@d2eOpTypeI _ _ _) (@d2eDstI _ _ _) (@d2eAddrI _ _ _) (@d2eValI _ _ _)
+                        (@d2eOpTypeI _ _ _) (@d2eDstI _ _ _) (@d2eAddrI _ _ _)
+                        (@d2eVal1I _ _ _) (@d2eVal2I _ _ _)
                         (@d2eRawInstI _ _ _) (@d2eCurPcI _ _ _) (@d2eNextPcI _ _ _)
-                        (@d2eEpochI _ _ _).
+                        (@d2eEpochI _ _ _)
+                        (@f2dPackI _ _) (@f2dRawInstI _ _) (@f2dCurPcI _ _)
+                        (@f2dNextPcI _ _) (@f2dEpochI _ _)
+                        (@e2wPackI _ _ _) (@e2wDecInstI _ _ _) (@e2wValI _ _ _).
 
-Definition p2stN := duplicate p2st lgNumChildren.
+Definition p4stN := duplicate p4st lgNumChildren.
 Definition memAtomic := memAtomic rv32iAddrSize fifoSize rv32iLgDataBytes lgNumChildren.
 
-Definition procMemAtomic := (p2stN ++ memAtomic)%kami.
+Definition procMemAtomic := (p4stN ++ memAtomic)%kami.
 
 (** MODIFY targetPgm to your target program *)
 Definition targetPgm := pgmFibonacci 10.
