examples/ProcFourStDec.v
@@ -1,0 +1,135 @@
+Require Import Bool String List.
+Require Import Lib.CommonTactics Lib.ilist Lib.Word.
+Require Import Lib.Struct Lib.StructNotation Lib.StringBound Lib.FMap Lib.StringEq Lib.Indexer.
+Require Import Kami.Syntax Kami.Semantics Kami.RefinementFacts Kami.Renaming Kami.Wf.
+Require Import Kami.Renaming Kami.Inline Kami.InlineFacts.
+Require Import Kami.Decomposition Kami.Notations Kami.Tactics Kami.ModuleBoundEx.
+Require Import Ex.MemTypes Ex.NativeFifo Ex.MemAtomic.
+Require Import Ex.SC Ex.ProcDec Ex.ProcThreeStage Ex.ProcThreeStDec Ex.ProcFDCorrect.
+Require Import Eqdep.
+
+Set Implicit Arguments.
+
+Section ProcFDE.
+  Variables addrSize lgDataBytes rfIdx: nat.
+
+  (* External abstract ISA: decoding and execution *)
+  Variables (getOptype: OptypeT lgDataBytes)
+            (getLdDst: LdDstT lgDataBytes rfIdx)
+            (getLdAddr: LdAddrT addrSize lgDataBytes)
+            (getLdSrc: LdSrcT lgDataBytes rfIdx)
+            (calcLdAddr: LdAddrCalcT addrSize lgDataBytes)
+            (getStAddr: StAddrT addrSize lgDataBytes)
+            (getStSrc: StSrcT lgDataBytes rfIdx)
+            (calcStAddr: StAddrCalcT addrSize lgDataBytes)
+            (getStVSrc: StVSrcT lgDataBytes rfIdx)
+            (getSrc1: Src1T lgDataBytes rfIdx)
+            (getSrc2: Src2T lgDataBytes rfIdx)
+            (getDst: DstT lgDataBytes rfIdx)
+            (exec: ExecT addrSize lgDataBytes)
+            (getNextPc: NextPcT addrSize lgDataBytes rfIdx)
+            (predictNextPc: forall ty, fullType ty (SyntaxKind (Bit addrSize)) -> (* pc *)
+                                       Expr ty (SyntaxKind (Bit addrSize))).
+
+  (* Abstract d2eElt *)
+  Variable (d2eElt: Kind).
+  Variable (d2ePack:
+              forall ty,
+                Expr ty (SyntaxKind (Bit 2)) -> (* opTy *)
+                Expr ty (SyntaxKind (Bit rfIdx)) -> (* dst *)
+                Expr ty (SyntaxKind (Bit addrSize)) -> (* addr *)
+                Expr ty (SyntaxKind (Data lgDataBytes)) -> (* val1 *)
+                Expr ty (SyntaxKind (Data lgDataBytes)) -> (* val2 *)
+                Expr ty (SyntaxKind (Data lgDataBytes)) -> (* rawInst *)
+                Expr ty (SyntaxKind (Bit addrSize)) -> (* curPc *)
+                Expr ty (SyntaxKind (Bit addrSize)) -> (* nextPc *)
+                Expr ty (SyntaxKind Bool) -> (* epoch *)
+                Expr ty (SyntaxKind d2eElt)).
+  Variables
+    (d2eOpType: forall ty, fullType ty (SyntaxKind d2eElt) ->
+                           Expr ty (SyntaxKind (Bit 2)))
+    (d2eDst: forall ty, fullType ty (SyntaxKind d2eElt) ->
+                        Expr ty (SyntaxKind (Bit rfIdx)))
+    (d2eAddr: forall ty, fullType ty (SyntaxKind d2eElt) ->
+                         Expr ty (SyntaxKind (Bit addrSize)))
+    (d2eVal1 d2eVal2: forall ty, fullType ty (SyntaxKind d2eElt) ->
+                                 Expr ty (SyntaxKind (Data lgDataBytes)))
+    (d2eRawInst: forall ty, fullType ty (SyntaxKind d2eElt) ->
+                            Expr ty (SyntaxKind (Data lgDataBytes)))
+    (d2eCurPc: forall ty, fullType ty (SyntaxKind d2eElt) ->
+                          Expr ty (SyntaxKind (Bit addrSize)))
+    (d2eNextPc: forall ty, fullType ty (SyntaxKind d2eElt) ->
+                           Expr ty (SyntaxKind (Bit addrSize)))
+    (d2eEpoch: forall ty, fullType ty (SyntaxKind d2eElt) ->
+                          Expr ty (SyntaxKind Bool)).
+
+  (* Abstract f2dElt *)  
+  Variable (f2dElt: Kind).
+  Variable (f2dPack:
+              forall ty,
+                Expr ty (SyntaxKind (Data lgDataBytes)) -> (* rawInst *)
+                Expr ty (SyntaxKind (Bit addrSize)) -> (* curPc *)
+                Expr ty (SyntaxKind (Bit addrSize)) -> (* nextPc *)
+                Expr ty (SyntaxKind Bool) -> (* epoch *)
+                Expr ty (SyntaxKind f2dElt)).
+  Variables
+    (f2dRawInst: forall ty, fullType ty (SyntaxKind f2dElt) ->
+                            Expr ty (SyntaxKind (Data lgDataBytes)))
+    (f2dCurPc: forall ty, fullType ty (SyntaxKind f2dElt) ->
+                          Expr ty (SyntaxKind (Bit addrSize)))
+    (f2dNextPc: forall ty, fullType ty (SyntaxKind f2dElt) ->
+                           Expr ty (SyntaxKind (Bit addrSize)))
+    (f2dEpoch: forall ty, fullType ty (SyntaxKind f2dElt) ->
+                          Expr ty (SyntaxKind Bool)).
+
+  (* Abstract e2wElt *)  
+  Variable (e2wElt: Kind).
+  Variable (e2wPack:
+              forall ty,
+                Expr ty (SyntaxKind d2eElt) -> (* decInst *)
+                Expr ty (SyntaxKind (Data lgDataBytes)) -> (* execVal *)
+                Expr ty (SyntaxKind e2wElt)).
+  Variables
+    (e2wDecInst: forall ty, fullType ty (SyntaxKind e2wElt) ->
+                            Expr ty (SyntaxKind d2eElt))
+    (e2wVal: forall ty, fullType ty (SyntaxKind e2wElt) ->
+                        Expr ty (SyntaxKind (Data lgDataBytes))).
+
+  Definition fetchDecode := ProcFetchDecode.fetchDecode
+                              getOptype getLdDst getLdAddr getLdSrc calcLdAddr
+                              getStAddr getStSrc calcStAddr getStVSrc
+                              getSrc1 getSrc2 getDst predictNextPc d2ePack
+                              f2dPack f2dRawInst f2dCurPc f2dNextPc f2dEpoch.
+
+  Definition p4st := (fetchDecode
+                        ++ regFile lgDataBytes rfIdx
+                        ++ scoreBoard rfIdx
+                        ++ oneEltFifo d2eFifoName d2eElt
+                        ++ oneEltFifoEx1 w2dFifoName (Bit addrSize)
+                        ++ (executer rfIdx exec d2eOpType d2eVal1 d2eVal2
+                                     d2eRawInst d2eCurPc e2wPack)
+                        ++ epoch
+                        ++ oneEltFifo e2wFifoName e2wElt
+                        ++ (wb "rqFromProc"%string "rsToProc"%string
+                               getNextPc d2eOpType d2eDst d2eAddr d2eVal1 d2eRawInst
+                               d2eCurPc d2eNextPc d2eEpoch e2wDecInst e2wVal))%kami.
+
+  Definition p3st := ProcThreeStage.p3st getOptype getLdDst getLdAddr getLdSrc calcLdAddr
+                                         getStAddr getStSrc calcStAddr getStVSrc
+                                         getSrc1 getSrc2 getDst exec getNextPc predictNextPc
+                                         d2ePack d2eOpType d2eDst d2eAddr d2eVal1 d2eVal2
+                                         d2eRawInst d2eCurPc d2eNextPc d2eEpoch
+                                         e2wPack e2wDecInst e2wVal.
+
+  Lemma p4st_refines_p3st: p4st <<== p3st.
+  Proof. (* SKIP_PROOF_ON
+    kmodular.
+    - kdisj_edms_cms_ex O.
+    - kdisj_ecms_dms_ex O.
+    - apply fetchDecode_refines_fetchNDecode.
+    - krefl.
+      END_SKIP_PROOF_ON *) admit.
+  Qed.
+
+End ProcFDE.
+
